GMAC spec structure

code/experimental/gcm/Hacl.Spec.GMAC.fst
@@ -4,14 +4,83 @@ module Spec = Spec.GF128
 
 open Spec
 
-open FStar.Mul
 open FStar.Seq
-open FStar.UInt8
 open FStar.Endianness
 
-noeq type gmac_state_ = | MkState: r:elem -> s:tag -> acc:elem -> pmsg:bytes{length pmsg < 16} -> gmac_state_
+type gmac_state_ = | MkState: r:elem -> acc:elem -> pmsg:bytes{length pmsg < 16} -> gmac_state_
 
-val gmac_init_spec: r:word_16 -> s:tag -> GTot gmac_state_
-let gmac_init_spec r s = MkState (encode r) s zero createEmpty
+#set-options "--z3rlimit 20 --initial_fuel 0 -0max_fuel 0 --initial_ifuel 0 --max_ifuel 0"
+
+let gmac_alloc_spec : gmac_state_ = MkState zero zero createEmpty
+
+val gmac_init_spec: r:key -> GTot gmac_state_
+let gmac_init_spec r = MkState (encode r) zero createEmpty
+
+val gmac_update_spec_nopmsg: cst:gmac_state_{length cst.pmsg = 0} -> msg:bytes ->
+  GTot gmac_state_ (decreases (length msg))
+let rec gmac_update_spec_nopmsg cst msg =
+  if length msg >= 16 then begin
+    let block : word = slice msg 0 16 in
+    let nmsg : bytes = slice msg 16 (length msg) in
+    let nacc = (cst.acc +@ (encode block)) *@ cst.r in
+    let nst = MkState cst.r nacc cst.pmsg in
+    gmac_update_spec_nopmsg nst nmsg
+  end else begin
+    MkState cst.r cst.acc msg
+  end
+
+val gmac_update_spec_wpmsg: cst:gmac_state_{length cst.pmsg > 0} -> msg:bytes ->
+  GTot gmac_state_
+let gmac_update_spec_wpmsg cst msg =
+  if length msg + length cst.pmsg >= 16 then begin
+    let block : word = cst.pmsg @| (slice msg 0 (16 - length cst.pmsg)) in
+    let nmsg : bytes = slice msg (16 - length cst.pmsg) (length msg) in
+    let nacc = (cst.acc +@ (encode block)) *@ cst.r in
+    let nst = MkState cst.r nacc createEmpty in
+    gmac_update_spec_nopmsg nst nmsg
+  end else begin
+    MkState cst.r cst.acc (cst.pmsg @| msg)
+  end
 
 val gmac_update_spec: cst:gmac_state_ -> msg:bytes -> GTot gmac_state_
+let gmac_update_spec cst msg =
+  if length cst.pmsg = 0 then gmac_update_spec_nopmsg cst msg
+  else gmac_update_spec_wpmsg cst msg
+
+val gmac_last_spec: cst:gmac_state_ -> GTot gmac_state_
+let gmac_last_spec cst =
+  let block : word = pad cst.pmsg in
+  let nacc = (cst.acc +@ (encode block)) *@ cst.r in
+  MkState cst.r nacc createEmpty
+
+val gmac_finish_spec: cst:gmac_state_ -> s:tag -> GTot tag
+let gmac_finish_spec cst s =
+  let nst = gmac_last_spec cst in
+  let nacc = (nst.acc +@ (encode s)) *@ nst.r in
+  decode nacc
+
+val gmac_spec: msg:bytes -> r:key -> s:tag -> 
+  GTot (t:tag{t = mac (encode_bytes msg) (encode r) s})
+let gmac_spec msg r s =
+  admit();
+  let st = gmac_init_spec r in
+  let st = gmac_update_spec st msg in
+  gmac_finish_spec st s
+  
+
+val flatten_bytes: msgs:seq bytes -> Tot bytes (decreases (length msgs))
+let rec flatten_bytes msgs =
+  if length msgs = 0 then createEmpty
+  else (head msgs) @| (flatten_bytes (tail msgs))
+  
+val gmac_update_spec_repeat: cst:gmac_state_ -> msgs:seq bytes -> GTot gmac_state_ (decreases (length msgs))
+let rec gmac_update_spec_repeat cst msgs =
+  if length msgs = 0 then cst
+  else
+    let nst = gmac_update_spec cst (head msgs) in
+    gmac_update_spec_repeat nst (tail msgs)
+    
+val lemma_gmac_update: st:gmac_state_ -> msgs:seq bytes -> Lemma
+  (requires True)
+  (ensures (gmac_update_spec_repeat st msgs = gmac_update_spec st (flatten_bytes msgs)))
+let lemma_gmac_update st msgs = admit()
